Fix up i2c_core verification top level and connect to i2c_reg_top proofs
The induction was replaced with mk_circuit_cstep; I also brought in the
`*_flat` trick from the i2c_reg_top verification, although I haven't
applied it everywhere.

common/shallowFlattenLib.sml
@@ -1,0 +1,90 @@
+(* A library for flattening a shallowly-embedded Verilog process (resolving the
+ * value of each field, and proving that it returns the input record with those
+ * fields updated to their new values). *)
+structure shallowFlattenLib =
+struct
+
+open HolKernel Parse boolLib bossLib;
+open combinSyntax TypeBase;
+
+val COND_2RAND = Q.prove (`
+  !f b x y z w.
+  f (if b then x else z) (if b then y else w) =
+  (if b then f x y else f z w)
+`,
+  Cases_on `b` >> simp []
+);
+
+val COND_2RAND_K = Q.prove (`
+  !f b x y z w.
+  f (K (if b then x else z)) (if b then y else w) =
+  (if b then f (K x) y else f (K z) w)
+`,
+  Cases_on `b` >> simp []
+);
+
+(* A version of TypeBase.fields_of which uses the concrete input type rather
+ * than the generalised one. *)
+fun fields_of_concrete (rty: hol_type) = map (fn (name, {accessor, fupd, ty}) => let
+  val accessor' = inst (match_type (accessor |> type_of |> dom_rng |> fst) rty) accessor;
+  val fupd' = inst (match_type (fupd |> type_of |> dom_rng |> snd) (rty --> rty)) fupd;
+  val ty' = accessor' |> type_of |> dom_rng |> snd;
+in
+  (name, {accessor = accessor', fupd = fupd', ty = ty'})
+end) (fields_of rty)
+
+fun prove_identity_fupds (rty: hol_type) = let
+  val fields = fields_of_concrete rty;
+  val nchotomy = nchotomy_of rty;
+in
+  (* TODO: may as well do one at a time now that we don't need to zip with the accessor/fupd theorems *)
+  LIST_CONJ (map (fn (_, {accessor, fupd, ty}) =>
+    prove (``!r. ^fupd (K (^accessor r)) r = r``,
+      gen_tac
+      >> qspec_then `r` strip_assume_tac nchotomy
+      >> first_x_assum (fn thm => pure_rewrite_tac [thm])
+      >> EVAL_TAC)
+  ) fields)
+end
+
+fun FORCE_FUPD_CONV ({accessor, fupd, ...}: rcd_fieldinfo) (tm: term) = let
+  val (f, _) = strip_comb tm;
+in
+  if term_eq f fupd then
+    raise UNCHANGED
+  else
+    prove (``^tm = ^fupd (K (^accessor ^tm)) ^tm``, pure_rewrite_tac [prove_identity_fupds (type_of tm)] >> REFL_TAC)
+end
+
+(* TODO: handle literal_case too *)
+fun COND_RECORD_CONV tm = DEPTH_CONV (fn tm =>
+  if is_cond tm andalso TypeBase.is_record_type (type_of tm) then let
+    val fields = type_of tm |> fields_of_concrete;
+    val (cond, thn, els) = dest_cond tm;
+    val (thn_f, thn_args) = strip_comb thn;
+    val (els_f, els_args) = strip_comb els;
+    val info = get_first (fn (_, info as {fupd, ...}) =>
+      if term_eq thn_f fupd orelse term_eq els_f fupd then
+        SOME info
+      else
+        NONE
+    ) fields;
+  in case info of
+      SOME (info as {fupd, ...}) =>
+        (LAND_CONV (QCONV (FORCE_FUPD_CONV info))
+        THENC RAND_CONV (QCONV (FORCE_FUPD_CONV info))
+        THENC (if (not $ term_eq thn_f fupd orelse is_K_1 (el 1 thn_args))
+          andalso (not $ term_eq els_f fupd orelse is_K_1 (el 1 els_args))
+        then
+          REWR_CONV (GSYM COND_2RAND_K)
+        else
+          REWR_CONV (GSYM COND_2RAND))
+        (* Make sure the new ifs we've just generated are covered too (and also clean up
+         * any needless ones). *)
+        THENC (LAND_CONV (REWR_CONV COND_ID ORELSEC COND_RECORD_CONV))
+        THENC (RAND_CONV (REWR_CONV COND_ID ORELSEC COND_RECORD_CONV))) tm
+    | NONE => raise UNCHANGED
+  end else
+    raise UNCHANGED) tm
+
+end
